Add map2, map3, zip, zip3, first_N to List.Tot.Base and some lemma

ulib/FStar.List.Tot.Base.fst
@@ -390,6 +390,69 @@ let rec unzip3 l = match l with
        let (tl1,tl2,tl3) = unzip3 tl in
        (hd1::tl1,hd2::tl2,hd3::tl3)
 
+(** [map2] takes a pair of list of the same length [x1; ...; xn] [y1; ... ; yn]
+ and return the list [f x1 y1 ; ... ; f xn yn ] *)
+val map2 (#a1 #a2 #b: Type)
+  (f: a1 -> a2 -> b)
+  (l1:list a1)
+  (l2:list a2)
+  : Pure (list b)
+    (requires (length l1 == length l2))
+    (ensures (fun _ -> True))
+    (decreases l1)
+let rec map2 #a1 #a2 #b f l1 l2 =
+  match l1, l2 with
+  | [], [] -> []
+  | x1::xs1, x2::xs2 -> f x1 x2 :: map2 f xs1 xs2
+
+(** [map2] takes three lists of the same length [x1; ...; xn]
+    [y1; ... ; yn] [z1; ... ; zn] and return the list
+    [f x1 y1 z1 ; ... ; f xn yn zn ] *)
+val map3 (#a1 #a2 #a3 #b: Type)
+  (f: a1 -> a2 -> a3 -> b)
+  (l1:list a1)
+  (l2:list a2)
+  (l3:list a3)
+  : Pure (list b)
+    (requires (let n = length l1 in
+      (n == length l2 /\
+        n == length l3)))
+    (ensures (fun _ -> True))
+    (decreases l1)
+let rec map3 #a1 #a2 #a3 #b f l1 l2 l3 =
+  match l1, l2, l3 with
+  | [], [], [] -> []
+  | x1::xs1, x2::xs2, x3::xs3 -> f x1 x2 x3 :: map3 f xs1 xs2 xs3
+
+(** [zip] takes a pair of list of the same length and returns
+    the list of index-wise pairs *)
+val zip (#a1 #a2:Type) (l1:list a1) (l2:list a2)
+  : Pure (list (a1 * a2))
+    (requires (let n = length l1 in n == length l2))
+    (ensures (fun _ -> True))
+let zip #a1 #a2 l1 l2 = map2 (fun x y -> x, y) l1 l2
+
+(** [zip3] takes a 3-tuple of list of the same length and returns
+    the list of index-wise 3-tuples *)
+val zip3 (#a1 #a2 #a3:Type) (l1:list a1) (l2:list a2) (l3:list a3)
+  : Pure (list (a1 * a2 * a3))
+    (requires (let n = length l1 in n == length l2 /\ n == length l3))
+    (ensures (fun _ -> True))
+let zip3 #a1 #a2 #a3 l1 l2 l3 = map3 (fun x y z -> x,y,z) l1 l2 l3
+
+
+(** Splitting a list at some index **)
+
+(** [first_N] takes a natural number n and a list and returns a pair
+    of the maximal prefix of l of size smaller than n and the rest of
+    the list *)
+let rec first_N (#a:Type) (n:nat) (l:list a) : list a * list a =
+  if n = 0 then [], l
+  else
+    match l with
+    | [] -> [], l
+    | x :: xs -> let l1, l2 = first_N (n-1) xs in x :: l1, l2
+
 (** Sorting (implemented as quicksort) **)
 
 (** [partition] splits a list [l] into two lists, the sum of whose
@@ -422,7 +485,7 @@ if, x > y. Requires, at type-checking time, [rel] to be a pure total
 function.  *)
 val compare_of_bool : #a:eqtype -> (a -> a -> Tot bool) -> a -> a -> Tot int
 let compare_of_bool #a rel x y =
-  if x `rel` y  then 1 
+  if x `rel` y  then 1
   else if x = y then 0
   else 0-1
 
