ulib/FStar.List.Tot.Properties.fst
@@ -852,3 +852,44 @@ let assoc_precedes
   (ensures (x << l /\ y << l))
 = assoc_memP_some x y l;
   memP_precedes (x, y) l
+
+(** Properties of first_N *)
+
+let rec first_N_length (#a:Type) (n:nat) (l:list a)
+  : Lemma (requires True) (ensures begin
+      let l_1, l_2 = first_N n l in
+      if length l < n then
+        length l_1 == length l /\ length l_2 == 0
+      else
+        length l_1 == n /\ length l_2 = length l - n
+    end)
+    (decreases n)
+=
+  if n = 0 then ()
+  else
+    match l with
+    | [] -> ()
+    | _::xs -> first_N_length (n-1) xs
+
+let rec first_N_assoc (#a:Type) (n1 n2:nat) (l:list a) : Lemma (requires True)
+  (ensures begin
+    let l1, l2 = first_N n1 l in
+    let l2, l3 = first_N n2 l2 in
+    let l1', l2' = first_N (n1+n2) l in
+    l1' ==  l1 @ l2 /\ l2' == l3
+    end)
+    (decreases n1)
+=
+  if n1 = 0 then ()
+  else
+    match l with
+    | [] -> ()
+    | x :: xs -> first_N_assoc (n1-1) n2 xs
+
+
+let rec first_N_length_total (#a:Type) (l:list a)
+  : Lemma (requires True) (ensures (first_N (length l) l == (l, []))) (decreases l)
+=
+  match l with
+  | [] -> ()
+  | x :: xs -> first_N_length_total xs
